updates

lib/adt/BinaryTree.dfy
@@ -50,14 +50,16 @@ module BinaryTree {
     {
     }
 
-    function Mirror<T>(t: Tree<T>) : Tree<T>
-    //ensures size(t) == size(mirror(t));
-    //ensures depth(t) == depth(mirror(t));
-    //ensures equal?(t, mirror(mirror(t)));
+    function method Mirror<T>(t: Tree<T>) : Tree<T>
     {
         match t
         case Nil => Nil
         case Node(x, l, r) => Node(x, Mirror(r), Mirror(l))
+    }
+
+    lemma MirrorEq<T>(t: Tree<T>)
+    ensures Equal?(t, Mirror(Mirror(t)))
+    {
     }
 
     lemma MirrorPerm<T>(t: Tree<T>)
