leetcode/0226-invert-binary-tree.dfy
@@ -1,0 +1,31 @@
+// Author: Shaobo He
+include "../lib/adt/BinaryTree.dfy"
+
+import opened BinaryTree
+
+function method Mirror<T>(t: Tree<T>) : Tree<T>
+{
+    match t
+    case Nil => Nil
+    case Node(x, l, r) => Node(x, Mirror(r), Mirror(l))
+}
+
+// TODO: figure out why post condition doesn't work
+lemma MirrorEq<T>(t: Tree<T>)
+ensures Equal?(t, Mirror(Mirror(t)))
+{
+}
+
+lemma MirrorPerm<T>(t: Tree<T>)
+ensures forall x :: CountBT(x, t) == CountBT(x, Mirror(t))
+{
+}
+    /*
+    match root
+    case Nil =>
+        mirror := Nil;
+    case Node(x, l, r) =>
+        var il := invertTree(r);
+        var ir := invertTree(l);
+        mirror := Node(x, il, ir);
+    */
